Foundation/Modal/Kripke2/K.lean
@@ -1,16 +1,37 @@
 import Foundation.Modal.Hilbert2.K
 import Foundation.Modal.Kripke2.Soundness
 import Foundation.Modal.Kripke2.Completeness
+import Foundation.Modal.Kripke2.Filteration
+import Foundation.Modal.Kripke2.FiniteFrame
 
 namespace LO.Modal
 
+open Kripke
+
 namespace Hilbert.K
 
-instance : System.Consistent (Hilbert.K) := Kripke.Hilbert.instConsistent Kripke.AllFrameClass
+instance : System.Consistent (Hilbert.K) := Hilbert.instConsistent AllFrameClass
 
-instance : Kripke.Canonical (Hilbert.K) (Kripke.AllFrameClass) := ⟨by trivial⟩
+instance : Kripke.Canonical (Hilbert.K) (AllFrameClass) := ⟨by trivial⟩
 
-instance : Complete (Hilbert.K) (Kripke.AllFrameClass) := inferInstance
+instance Kripke.CompleteAll : Complete (Hilbert.K) (AllFrameClass) := inferInstance
+
+instance Kripke.CompleteAllFinite : Complete (Hilbert.K) (AllFiniteFrameClass) := ⟨by
+  intro φ hp;
+  apply Kripke.CompleteAll.complete;
+  intro F _ V x;
+  let M : Kripke.Model := ⟨F, V⟩;
+  let FM := coarsestFilterationModel M ↑φ.subformulas;
+
+  apply filteration FM (coarsestFilterationModel.filterOf) (by aesop) |>.mpr;
+  apply hp (by
+    suffices Finite (FilterEqvQuotient M φ.subformulas) by
+      simp only [FiniteFrameClass.toFrameClass, AllFiniteFrameClass, Set.image_univ, Set.mem_range];
+      tauto;
+    apply FilterEqvQuotient.finite;
+    simp;
+  ) FM.Val
+⟩
 
 end Hilbert.K
 
